SystemFD/Evaluator/Soundness.lean
@@ -1,0 +1,128 @@
+import SystemFD.Term
+import SystemFD.Reduction
+import SystemFD.Ctx
+import SystemFD.Evaluator
+import SystemFD.Algorithm
+import SystemFD.Judgment
+
+theorem eval_inst_soundess : eval_inst Γ t = .some ts -> Red Γ t ts := by
+intros
+induction Γ, t using eval_inst.induct generalizing ts
+case _ Γ =>
+  sorry
+case _ t Γ n sp head A t' f et =>
+  induction sp
+  case _ =>
+    have t' := Term.spine_lemma head; symm at head;
+    simp at t'; subst t'; simp at et; rw [f] at et; simp at et; symm at et; subst et;
+    symm at f; apply Red.letterm_nil head f; rfl
+  case _ =>
+    have t' := Term.spine_lemma head; symm at head; symm at f;
+
+     sorry
+case _ t Γ n sp head no nt et =>
+  have t' := Term.spine_lemma head; subst t';
+  sorry
+case _ Γ a b f _ et => simp at et; subst et; apply Red.beta
+case _ Γ a b et =>
+  simp at et; subst et; apply Red.betat
+case _ Γ f t _ nf ih1 et =>
+  -- have ih := @ih1 (f `@ t) et wf;
+  simp at et; have fnf := Term.neutral_form_app nf;
+
+  sorry
+case _ ih et =>
+  simp at et;
+  sorry
+case _ => sorry
+case _ => sorry
+case _ Γ _ _ ih => simp at ih; rw[<-ih]; apply Red.sym
+case _ ih η =>
+  simp at η; rw[Option.bind_eq_some] at η
+  cases η; case _ w η' =>
+    have ih' := @ih w (And.left η');
+    injection (And.right η') with ts'; symm at ts'; subst ts';
+    apply Red.sym_congr ih'; rfl
+
+case _ Γ t t' teq nf ih =>
+  have e := eq_of_beq teq; subst e;
+  simp at ih; rw [<-ih]; exact Red.seq
+case _ Γ t' t h x ih =>
+  simp at ih; have nh := And.left ih; exfalso;
+  contradiction
+case _ Γ t t' t'' teq x et=>
+  have eq := eq_of_beq teq; subst eq;
+  simp at et; rw[<-et]; exact Red.appc
+case _ Γ t t' t'' teq x et=>
+  simp at et; have nh := And.left et; contradiction
+
+case _ Γ A B _ et => simp at et; subst et; apply Red.fst
+case _ _ _ _ _ et => simp at et; subst et; apply Red.snd
+case _ et => simp at et; subst et; apply Red.arrowc
+case _ Γ t η _ _ ih et =>
+  simp at et; rw[Option.bind_eq_some] at et;
+  cases et; case _ η' h =>
+  have ih' := @ih η' (And.left h);
+  injection (And.right h) with w; subst w;
+  apply Red.arrowc_congr2 ih'; rfl
+case _ ih et =>
+  simp at et; rw[Option.bind_eq_some] at et;
+  cases et; case _ η' h =>
+  have ih' := @ih η' (And.left h);
+  injection (And.right h) with w; subst w;
+  apply Red.arrowc_congr1 ih'; rfl
+case _ et => simp at et; subst et; apply Red.allc
+case _ Γ t η _ _ ih1 et=>
+  simp at et; rw[Option.bind_eq_some] at et;
+  cases et; case _ w h =>
+    have ih := @ih1 w (And.left h);
+    injection (And.right h) with w;
+    subst w; apply Red.allc_congr ih; rfl
+
+case _ Γ t a _ ih=>
+  simp at ih; rw[<-ih]; exact Red.cast
+case _ Γ t η x _ ih1 ih=>
+  simp at ih; rw[Option.bind_eq_some] at ih;
+  cases ih; case _ h w =>
+    have h' := And.right w; injection h' with w';
+    have qq := @ih1 h (And.left w)
+    rw [<-w']; apply Red.cast_congr qq; rfl
+case _ Γ t K _ ih et =>
+  simp at et; rw[Option.bind_eq_some] at et;
+  cases et; case _ w h =>
+  have ih' := @ih w (And.left h);
+  injection (And.right h) with w; subst w
+  apply Red.letdata_congr ih'; rfl
+case _ Γ A t t' _ ih et  =>
+  simp at et; rw[Option.bind_eq_some] at et;
+  cases et; case _ w h =>
+  have ih' := @ih w (And.left h);
+  injection (And.right h) with w; subst w
+  apply Red.letterm_congr ih'; rfl
+case _ Γ t t' _ ih et =>
+  simp at et; rw[Option.bind_eq_some] at et;
+  cases et; case _ w h =>
+  have ih' := @ih w (And.left h);
+  injection (And.right h) with w; subst w;
+  apply Red.letctor_congr ih'; rfl
+case _ ih et =>
+  simp at et; rw[Option.bind_eq_some] at et;
+  cases et; case _ w h =>
+  have ih' := @ih w (And.left h);
+  injection (And.right h) with w; subst w;
+  apply Red.letopentype_congr ih'; rfl
+case _ ih et =>
+  simp at et; rw[Option.bind_eq_some] at et;
+  cases et; case _ w h =>
+  have ih' := @ih w (And.left h);
+  injection (And.right h) with w; subst w;
+  apply Red.letopen_congr ih'; rfl
+case _ ih et =>
+  simp at et; rw[Option.bind_eq_some] at et;
+  cases et; case _ w h =>
+  have ih' := @ih w (And.left h);
+  injection (And.right h) with w; subst w;
+  apply Red.insttype_congr ih'; rfl
+case _ tnone _ _ _ _ _ _ _ _ _ _ _ _ _  _ _ _  _ _ _ _ _ _ _ _ _ et =>
+  simp at et; rw [tnone] at et;
+  simp at et
