SystemFD/Soundness/Preservation.lean
@@ -1,0 +1,7 @@
+import SystemFD.Term
+import SystemFD.Judgment
+import SystemFD.Ctx
+import SystemFD.Algorithm
+import SystemFD.Reduction
+
+theorem preservation : ⊢ Γ -> Γ ⊢ t : A -> Red Γ t ts := sorry
