README.md
@@ -1,1 +1,14 @@
 # SystemFD
+
+- Terms: Terms of the language
+- Evaulator: evaluates terms
+- Algoritm: typecheck terms
+
+- Reduction : Specification for reduction
+- Judgements: Specification of type checking
+
+
+This formalization proves:
+- [ ] Soundness of type checking with respect to type checking judgements
+- [ ] Soundness of evaluation with respect to reduction semantics
+- [ ] Progress and preservation
